json/Theorems/Utf8DFA.v
@@ -1,0 +1,366 @@
+From Coq Require Import Strings.Byte.
+
+
+Require Import Json.Parser.
+Require Import Json.Utf8.
+Require Import Json.Utf8DFA.
+Require Import Json.Theorems.Parser.
+Require Import Json.Theorems.Utf8.
+From Coq Require Import Lists.List. Import ListNotations.
+From Coq Require Import Lia.
+
+Local Notation "0" := false.
+Local Notation "1" := true.
+Definition zero_codep : codepoint := (0, b4_zero, b4_zero, b4_zero, b4_zero, b4_zero).
+
+Lemma byte_range_00_7f_bits : forall b,
+    byte_range b = Range_00_7F ->
+    exists b1 b2 b3 b4 b5 b6 b7,
+      Byte.to_bits b = (b1, (b2, (b3, (b4, (b5, (b6, (b7, 0))))))).
+Proof.
+  intros.
+  destruct b; inversion H; repeat eexists.
+Qed.
+
+Lemma byte_range_80_8f_bits : forall b,
+    byte_range b = Range_80_8F ->
+    exists b1 b2 b3 b4,
+      Byte.to_bits b = (b1, (b2, (b3, (b4, (0, (0, (0, 1))))))).
+Proof.
+  intros.
+  destruct b; inversion H; repeat eexists.
+Qed.
+
+Lemma byte_range_90_9f_bits : forall b,
+    byte_range b = Range_90_9F ->
+    exists b1 b2 b3 b4,
+      Byte.to_bits b = (b1, (b2, (b3, (b4, (1, (0, (0, 1))))))).
+Proof.
+  intros.
+  destruct b; inversion H; repeat eexists.
+Qed.
+
+Lemma byte_range_a0_bf_bits : forall b,
+    byte_range b = Range_A0_BF ->
+    exists b1 b2 b3 b4 b5,
+      Byte.to_bits b = (b1, (b2, (b3, (b4, (b5, (1, (0, 1))))))).
+Proof.
+  intros.
+  - destruct b; inversion H; repeat eexists.
+Qed.
+
+Lemma byte_range_c0_c1_bits : forall b,
+    byte_range b = Range_C0_C1 ->
+    exists b1,
+      Byte.to_bits b = (b1, (0, (0, (0, (0, (0, (1, 1))))))).
+Proof.
+  intros.
+  destruct b; inversion H; repeat eexists.
+Qed.
+
+Lemma byte_range_c2_df_bits : forall b,
+    byte_range b = Range_C2_DF ->
+    exists b1 b2 b3 b4 b5,
+      (Byte.to_bits b = (b1, (b2, (b3, (b4, (b5, (0, (1, 1))))))) /\
+       (b3 = 0 /\ b4 = 0 /\ b5 = 0 -> b2 = 1)).
+Proof.
+  intros.
+  destruct b; inversion H; repeat eexists; intros G; destruct G as [P1 [P2 P3]]; try discriminate; reflexivity.
+Qed.
+
+Lemma byte_e0_bits : forall b,
+    byte_range b = Byte_E0 ->
+    (Byte.to_bits b = (0, (0, (0, (0, (0, (1, (1, 1)))))))).
+Proof.
+  intros.
+  destruct b; inversion H; reflexivity.
+Qed.
+
+Lemma byte_range_e1_ef_bits : forall b,
+    byte_range b = Range_E1_EF ->
+    exists b1 b2 b3 b4,
+      Byte.to_bits b = (b1, (b2, (b3, (b4, (0, (1, (1, 1))))))).
+Proof.
+  intros.
+  destruct b; inversion H; repeat eexists.
+Qed.
+
+Lemma byte_f0_bits : forall b,
+    byte_range b = Byte_F0 ->
+    Byte.to_bits b = (0, (0, (0, (0, (1, (1, (1, 1))))))).
+Proof.
+  intros.
+  destruct b; inversion H; reflexivity.
+Qed.
+
+
+Lemma byte_range_f1_f3_bits : forall b,
+    byte_range b = Range_F1_F3 ->
+    exists b1 b2,
+      Byte.to_bits b = (b1, (b2, (0, (0, (1, (1, (1, 1))))))).
+Proof.
+  intros.
+  destruct b; inversion H; repeat eexists.
+Qed.
+
+Lemma byte_f4_bits : forall b,
+    byte_range b = Byte_F4 ->
+    Byte.to_bits b = (0, (0, (1, (0, (1, (1, (1, 1))))))).
+Proof.
+  intros.
+  destruct b; inversion H; reflexivity.
+Qed.
+
+
+Lemma byte_range_f5_ff_bits : forall b,
+    byte_range b = Range_F5_FF ->
+    exists b1 b2 b3 b4,
+      Byte.to_bits b = (b1, (b2, (b3, (b4, (1, (1, (1, 1))))))).
+Proof.
+  intros.
+  destruct b; inversion H; repeat eexists.
+Qed.
+
+
+Lemma byte_range_of_bits_a0_bf: forall b1 b2 b3 b4 b5,
+    byte_range (of_bits (b1, (b2, (b3, (b4, (b5, (1, (0, 1)))))))) = Range_A0_BF.
+Proof.
+  intros.
+  destruct (of_bits (b1, (b2, (b3, (b4, (b5, (1, (0, 1)))))))) eqn:H;
+    apply (f_equal Byte.to_bits) in H;
+    rewrite Byte.to_bits_of_bits in H;
+    inversion H;
+    reflexivity.
+Qed.
+
+Lemma byte_range_of_bits_80_8f: forall (b1 b2 b3 b4: bool),
+    byte_range (of_bits (b1, (b2, (b3, (b4, (0, (0, (0, 1)))))))) = Range_80_8F.
+Proof.
+  intros.
+  destruct (of_bits (b1, (b2, (b3, (b4, (0, (0, (0, 1)))))))) eqn:H;
+    apply (f_equal Byte.to_bits) in H;
+    rewrite Byte.to_bits_of_bits in H;
+    inversion H;
+    auto.
+Qed.
+
+Lemma byte_range_of_bits_80_bf: forall (b1 b2 b3 b4 b5 b6: bool),
+    let b := of_bits (b1, (b2, (b3, (b4, (b5, (b6, (0, 1))))))) in
+    (byte_range b = Range_80_8F) \/
+      (byte_range b = Range_90_9F) \/
+      (byte_range b = Range_A0_BF).
+Proof.
+  intros.
+  destruct b eqn:H;
+    apply (f_equal Byte.to_bits) in H;
+    subst b;
+    rewrite Byte.to_bits_of_bits in H;
+    inversion H;
+    auto.
+Qed.
+
+Lemma byte_range_of_bits_90_9f: forall (b1 b2 b3 b4: bool),
+    let b := of_bits (b1, (b2, (b3, (b4, (1, (0, (0, 1))))))) in
+    (byte_range b = Range_90_9F).
+Proof.
+  intros.
+  destruct b eqn:H;
+    apply (f_equal Byte.to_bits) in H;
+    subst b;
+    rewrite Byte.to_bits_of_bits in H;
+    inversion H;
+    auto.
+Qed.
+
+Lemma next_state_expecting_1_80_bf :
+  forall c1 c2 c3 c4 c5 c6
+    b1 b2 b3 b4 b5 b6 b7 b8 b9 b10 b11 b12 b13 b14 b15 b16 b17 b18 b19 b20 b21,
+    let b := (of_bits (b21, (b20, (b19, (b18, (b17, (b16, (0, 1)))))))) in
+    next_state Expecting_1_80_BF (c1, (c2, c3, c4, c5), (c6, b1, b2, b3), (b4, b5, b6, b7), (b8, b9, b10, b11), (b12, b13, b14, b15)) b
+    = Ok (Finished (b1, (b2, b3, b4, b5), (b6, b7, b8, b9), (b10, b11, b12, b13), (b14, b15, b16, b17), (b18, b19, b20, b21))).
+Proof.
+  intros.
+  unfold next_state. subst b.
+  pose proof (byte_range_of_bits_80_bf b21 b20 b19 b18 b17 b16) as [G | [G | G]]; rewrite G;
+    unfold push_bottom_bits;
+    rewrite Byte.to_bits_of_bits; reflexivity.
+Qed.
+
+Lemma next_state_expecting_2_80_bf :
+  forall c1 c2 c3 c4 c5 c6
+    b1 b2 b3 b4 b5 b6 b7 b8 b9 b10 b11 b12 b13 b14 b15 b16 b17 b18 b19 b20 b21,
+    let b := (of_bits (b21, (b20, (b19, (b18, (b17, (b16, (0, 1)))))))) in 
+    next_state Expecting_2_80_BF (c1, (c2, c3, c4, c5), (c6, b1, b2, b3), (b4, b5, b6, b7), (b8, b9, b10, b11), (b12, b13, b14, b15)) b
+    = Ok (More Expecting_1_80_BF (b1, (b2, b3, b4, b5), (b6, b7, b8, b9), (b10, b11, b12, b13), (b14, b15, b16, b17), (b18, b19, b20, b21))).
+Proof.
+  intros.
+  unfold next_state. subst b.
+  pose proof (byte_range_of_bits_80_bf b21 b20 b19 b18 b17 b16) as [G | [G | G]]; rewrite G;
+    unfold push_bottom_bits;
+    rewrite Byte.to_bits_of_bits; reflexivity.
+Qed.
+
+
+Lemma next_state_expecting_3_80_bf :
+  forall c1 c2 c3 c4 c5 c6
+    b1 b2 b3 b4 b5 b6 b7 b8 b9 b10 b11 b12 b13 b14 b15 b16 b17 b18 b19 b20 b21,
+    let b := (of_bits (b21, (b20, (b19, (b18, (b17, (b16, (0, 1)))))))) in 
+    next_state Expecting_3_80_BF (c1, (c2, c3, c4, c5), (c6, b1, b2, b3), (b4, b5, b6, b7), (b8, b9, b10, b11), (b12, b13, b14, b15)) b
+    = Ok (More Expecting_2_80_BF (b1, (b2, b3, b4, b5), (b6, b7, b8, b9), (b10, b11, b12, b13), (b14, b15, b16, b17), (b18, b19, b20, b21))).
+Proof.
+  intros.
+  unfold next_state. subst b.
+  pose proof (byte_range_of_bits_80_bf b21 b20 b19 b18 b17 b16) as [G | [G | G]]; rewrite G;
+    unfold push_bottom_bits;
+    rewrite Byte.to_bits_of_bits; reflexivity.
+Qed.
+
+Lemma next_state_expecting_3_80_8f :
+  forall c1 c2 c3 c4 c5 c6
+    b1 b2 b3 b4 b5 b6 b7 b8 b9 b10 b11 b12 b13 b14 b15 b18 b19 b20 b21,
+    let b := (of_bits (b21, (b20, (b19, (b18, (0, (0, (0, 1)))))))) in
+    next_state Expecting_3_80_8F (c1, (c2, c3, c4, c5), (c6, b1, b2, b3), (b4, b5, b6, b7), (b8, b9, b10, b11), (b12, b13, b14, b15)) b
+    = Ok (More Expecting_2_80_BF (b1, (b2, b3, b4, b5), (b6, b7, b8, b9), (b10, b11, b12, b13), (b14, b15, 0, 0), (b18, b19, b20, b21))).
+Proof.
+  intros.
+  unfold next_state. subst b.
+  pose proof (byte_range_of_bits_80_8f b21 b20 b19 b18) as G.
+  rewrite G.
+  unfold push_bottom_bits.
+  rewrite Byte.to_bits_of_bits. reflexivity.
+Qed.
+
+Lemma next_state_expecting_3_90_bf_p1 :
+  forall c1 c2 c3 c4 c5 c6
+    b1 b2 b3 b4 b5 b6 b7 b8 b9 b10 b11 b12 b13 b14 b15 b17 b18 b19 b20 b21,
+    let b := (of_bits (b21, (b20, (b19, (b18, (b17, (1, (0, 1)))))))) in 
+    next_state Expecting_3_90_BF (c1, (c2, c3, c4, c5), (c6, b1, b2, b3), (b4, b5, b6, b7), (b8, b9, b10, b11), (b12, b13, b14, b15)) b
+    = Ok (More Expecting_2_80_BF (b1, (b2, b3, b4, b5), (b6, b7, b8, b9), (b10, b11, b12, b13), (b14, b15, 1, b17), (b18, b19, b20, b21))).
+Proof.
+  intros.
+  unfold next_state. subst b.
+  pose proof (byte_range_of_bits_a0_bf b21 b20 b19 b18 b17) as G.
+  rewrite G.
+  unfold push_bottom_bits.
+  rewrite Byte.to_bits_of_bits; reflexivity.
+Qed.
+
+Lemma next_state_expecting_3_90_bf_p2 :
+  forall c1 c2 c3 c4 c5 c6
+    b1 b2 b3 b4 b5 b6 b7 b8 b9 b10 b11 b12 b13 b14 b15 b18 b19 b20 b21,
+    let b := (of_bits (b21, (b20, (b19, (b18, (1, (0, (0, 1)))))))) in 
+    next_state Expecting_3_90_BF (c1, (c2, c3, c4, c5), (c6, b1, b2, b3), (b4, b5, b6, b7), (b8, b9, b10, b11), (b12, b13, b14, b15)) b
+    = Ok (More Expecting_2_80_BF (b1, (b2, b3, b4, b5), (b6, b7, b8, b9), (b10, b11, b12, b13), (b14, b15, 0, 1), (b18, b19, b20, b21))).
+Proof.
+  intros.
+  unfold next_state. subst b.
+  pose proof (byte_range_of_bits_90_9f b21 b20 b19 b18) as G; rewrite G;
+    unfold push_bottom_bits;
+    rewrite Byte.to_bits_of_bits; reflexivity.
+Qed.
+
+Lemma next_state_expecting_2_a0_bf :
+  forall c1 c2 c3 c4 c5 c6
+    b1 b2 b3 b4 b5 b6 b7 b8 b9 b10 b11 b12 b13 b14 b15 b17 b18 b19 b20 b21,
+    let b := (of_bits (b21, (b20, (b19, (b18, (b17, (1, (0, 1)))))))) in
+    next_state Expecting_2_A0_BF (c1, (c2, c3, c4, c5), (c6, b1, b2, b3), (b4, b5, b6, b7), (b8, b9, b10, b11), (b12, b13, b14, b15)) b
+    = Ok (More Expecting_1_80_BF (b1, (b2, b3, b4, b5), (b6, b7, b8, b9), (b10, b11, b12, b13), (b14, b15, 1, b17), (b18, b19, b20, b21))).
+Proof.
+  intros.
+  unfold next_state. subst b.
+  pose proof (byte_range_of_bits_a0_bf b21 b20 b19 b18 b17) as G. rewrite G.
+  unfold push_bottom_bits.
+  rewrite Byte.to_bits_of_bits. reflexivity.
+Qed.
+
+Lemma if_redundant : forall T (P: T) (b: bool), (if b then P else P) = P.
+Proof.
+  destruct b; reflexivity.
+Qed.
+
+Theorem utf8_decoders_equal_strong : forall (bytes less: list byte),
+    (List.length less) <= (List.length bytes) -> 
+    utf8_dfa_decode less = utf8_decode less.
+Proof.
+  Opaque Byte.of_bits.
+  intros bytes.
+  induction bytes; intros.
+  - inversion H. rewrite length_zero_iff_nil in H1. subst. reflexivity.
+  - unfold utf8_dfa_decode, utf8_decode, all, all_aux. fold (all_aux parse_codepoint).   
+    destruct less as [| byte byte_rest]; [ reflexivity | ]. 
+    destruct (parse_codepoint (byte :: byte_rest)) as [[val rest] | err] eqn:P_byte_byte_rest.
+    rewrite <- all_aux_saturation_aux with (n:= (S (S (Datatypes.length (rest))))).
+    fold (all parse_codepoint rest). fold (utf8_decode rest). rewrite <- IHbytes.
+    3: apply parse_codepoint_strong_progress.
+    2,3,4: simpl in H; apply parse_codepoint_strong_progress in P_byte_byte_rest; simpl in P_byte_byte_rest; simpl; lia.
+    simpl. 
+    unfold parse_codepoint, parse_header, encoding_size_from_header in P_byte_byte_rest.
+    unfold next_state, extract_3_bits, extract_4_bits, extract_5_bits, extract_7_bits.
+    destruct (byte_range byte) eqn:B; [
+        apply byte_range_00_7f_bits in B as byte_bits; destruct byte_bits as [b1 [b2 [b3 [b4 [b5 [b6 [b7 byte_bits]]]]]]]
+      | apply byte_range_80_8f_bits in B as byte_bits; destruct byte_bits as [b1 [b2 [b3 [b4 byte_bits]]]]
+      | apply byte_range_90_9f_bits in B as byte_bits; destruct byte_bits as [b1 [b2 [b3 [b4 byte_bits]]]]
+      | apply byte_range_a0_bf_bits in B as byte_bits; destruct byte_bits as [b1 [b2 [b3 [b4 [b5 byte_bits]]]]]
+      | apply byte_range_c0_c1_bits in B as byte_bits; destruct byte_bits as [b1 byte_bits]
+      | apply byte_range_c2_df_bits in B as byte_bits; destruct byte_bits as [b1 [b2 [b3 [b4 [b5 [byte_bits not_c0_c1]]]]]]
+      | apply byte_e0_bits in B as byte_bits
+      | apply byte_range_e1_ef_bits in B as byte_bits; destruct byte_bits as [b1 [b2 [b3 [b4 byte_bits]]]]
+      | apply byte_f0_bits in B as byte_bits
+      | apply byte_range_f1_f3_bits in B as byte_bits; destruct byte_bits as [b1 [b2 byte_bits]]
+      | apply byte_f4_bits in B as byte_bits
+      | apply byte_range_f5_ff_bits in B as byte_bits; destruct byte_bits as [b1 [b2 [b3 [b4 byte_bits]]]]
+      ]; rewrite byte_bits in *; simpl in *; try (crush_bits; simpl in *; inversion P_byte_byte_rest; subst; reflexivity).
+    * destruct (parse_continuation byte_rest) as [[r byte_rest2] | err]; try discriminate.
+    * repeat rewrite if_redundant in P_byte_byte_rest.
+      simpl in *; destruct (parse_continuation byte_rest) as [[r byte_rest2] | err] eqn:P_cont_byte_rest; try discriminate.
+      simpl in P_byte_byte_rest; to_bits r; inversion P_byte_byte_rest; subst.
+      destruct byte_rest; try discriminate;
+        destruct_parse_continuation; inversion P_cont_byte_rest; subst;
+        crush_bits; simpl; unfold b4_zero;
+        rewrite next_state_expecting_1_80_bf; simpl; inversion H1; subst; reflexivity.
+    * destruct (parse_continuation byte_rest) as [[snd rest2] | err] eqn:P_cont_byte_rest; try discriminate. simpl in P_byte_byte_rest.
+      destruct (parse_continuation rest2) as [[trd rest3] | err] eqn:P_cont_rest2; try discriminate. simpl in P_byte_byte_rest. to_bits snd; to_bits trd.
+      crush_bits; try discriminate.
+      repeat destruct_parse_continuation. inversion P_cont_byte_rest; inversion P_cont_rest2; inversion P_byte_byte_rest; subst.
+      simpl. unfold b4_zero. rewrite next_state_expecting_2_a0_bf. simpl.
+      rewrite next_state_expecting_1_80_bf. simpl. reflexivity.
+    * rewrite if_redundant in P_byte_byte_rest.
+      simpl in *.
+      destruct (parse_continuation byte_rest) as [[snd rest2] | err] eqn:P_cont_byte_rest; try discriminate. simpl in P_byte_byte_rest.
+      destruct (parse_continuation rest2) as [[trd rest3] | err] eqn:P_cont_rest2; try discriminate. simpl in P_byte_byte_rest. to_bits snd; to_bits trd.
+      repeat destruct_parse_continuation.
+      crush_bits; inversion P_cont_byte_rest; inversion P_cont_rest2; inversion P_byte_byte_rest; simpl; subst;
+      unfold b4_zero;
+      rewrite next_state_expecting_2_80_bf; simpl;
+      rewrite next_state_expecting_1_80_bf; reflexivity.
+    * destruct (parse_continuation byte_rest) as [[snd rest2] | err] eqn:P_cont_byte_rest; try discriminate. simpl in P_byte_byte_rest.
+      destruct (parse_continuation rest2) as [[trd rest3] | err] eqn:P_cont_rest2; try discriminate. simpl in P_byte_byte_rest. to_bits snd; to_bits trd.
+      destruct (parse_continuation rest3) as [[frth rest4] | err] eqn:P_cont_rest3; try discriminate. simpl in P_byte_byte_rest. to_bits frth.
+      crush_bits; simpl; repeat destruct_parse_continuation;
+        inversion P_cont_byte_rest; inversion P_cont_rest2; inversion P_cont_rest3; inversion P_byte_byte_rest; subst;
+        simpl; unfold b4_zero;
+        try rewrite next_state_expecting_3_90_bf_p1; try rewrite next_state_expecting_3_90_bf_p2; simpl;
+             rewrite next_state_expecting_2_80_bf; simpl;
+             rewrite next_state_expecting_1_80_bf; reflexivity.
+    * destruct (parse_continuation byte_rest) as [[snd rest2] | err] eqn:P_cont_byte_rest; try discriminate. simpl in P_byte_byte_rest.
+      destruct (parse_continuation rest2) as [[trd rest3] | err] eqn:P_cont_rest2; try discriminate. simpl in P_byte_byte_rest. to_bits snd; to_bits trd.
+      destruct (parse_continuation rest3) as [[frth rest4] | err] eqn:P_cont_rest3; try discriminate. simpl in P_byte_byte_rest. to_bits frth. unfold b4_zero.
+      crush_bits; simpl; repeat destruct_parse_continuation;
+        inversion P_cont_byte_rest; inversion P_cont_rest2; inversion P_cont_rest3; inversion P_byte_byte_rest; subst; simpl;
+        rewrite next_state_expecting_3_80_bf; simpl;
+        rewrite next_state_expecting_2_80_bf; simpl;
+        rewrite next_state_expecting_1_80_bf; reflexivity.
+     * destruct (parse_continuation byte_rest) as [[snd rest2] | err] eqn:P_cont_byte_rest; try discriminate. simpl in P_byte_byte_rest.
+      destruct (parse_continuation rest2) as [[trd rest3] | err] eqn:P_cont_rest2; try discriminate. simpl in P_byte_byte_rest. to_bits snd; to_bits trd.
+      destruct (parse_continuation rest3) as [[frth rest4] | err] eqn:P_cont_rest3; try discriminate. simpl in P_byte_byte_rest. to_bits frth. unfold b4_zero.
+      repeat destruct_parse_continuation.
+      crush_bits; try discriminate.
+        inversion P_cont_byte_rest; inversion P_cont_rest2; inversion P_cont_rest3; inversion P_byte_byte_rest; subst. simpl. unfold b4_zero.
+      rewrite next_state_expecting_3_80_8f; simpl;
+        rewrite next_state_expecting_2_80_bf; simpl;
+        rewrite next_state_expecting_1_80_bf; reflexivity.
+     * destruct byte; try discriminate B; inversion byte_bits; subst; simpl in P_byte_byte_rest;
+       destruct (parse_continuation byte_rest) as [[snd rest2] | err] eqn:P_cont_byte_rest; try discriminate; simpl in P_byte_byte_rest;
+      destruct (parse_continuation rest2) as [[trd rest3] | err] eqn:P_cont_rest2; try discriminate; simpl in P_byte_byte_rest; to_bits snd; to_bits trd;
+         destruct (parse_continuation rest3) as [[frth rest4] | err] eqn:P_cont_rest3; try discriminate.
+     * 
